WIP

src/tls/Extensions.fst
@@ -17,6 +17,8 @@ module TI = TLSInfo
  Define extension. 
  *************************************************)
 
+type obfuscated_ticket_age = lbytes 4  // should it be UInt32? 
+
 (** RFC 4.2 'Extension' Table's type definition. *)
 noeq type preEarlyDataIndication : Type0 =
   { ped_configuration_id: configurationId;
@@ -28,7 +30,6 @@ noeq type preEarlyDataIndication : Type0 =
 and earlyDataIndication =
   | ClientEarlyDataIndication of preEarlyDataIndication
   | ServerEarlyDataIndication
-
 (* SI: we currently only define Mandatory-to-Implement Extensions 
    as listed in the RFC's Section 8.2. Labels in the variants below are: 
      M  - "MUST implement"
@@ -49,7 +50,9 @@ and extension =
   | E_client_certificate_type 
   | E_padding *)
   | E_key_share of CommonDH.keyShare (* M, AF *)
-  | E_pre_shared_key of PSK.preSharedKey (* M, AF *)
+
+  // this is the truncated one
+  | E_pre_shared_key of list (PSK.preSharedKey * obfuscated_ticket_age)  (* M, AF *)
 (*| E_psk_key_exchange_modes *)
   | E_early_data of earlyDataIndication
   | E_cookie of b:bytes { 1 <= length b /\ length b <= ((pow2 16) - 1)}  (* M *)
@@ -445,7 +448,15 @@ private let rec list_valid_ng_is_list_ng (#p:(namedGroup -> Type)) (l:list (n:na
   | hd :: tl -> hd :: list_valid_ng_is_list_ng tl
 
 (* SI: API. Called by Handshake. *)
-val prepareExtensions: protocolVersion -> (k:valid_cipher_suites{List.Tot.length k < 256}) -> bool -> bool -> list sigHashAlg -> list (x:namedGroup{SEC? x \/ FFDHE? x}) -> option (TI.cVerifyData * TI.sVerifyData) -> (option CommonDH.keyShare) -> Tot (l:list extension{List.Tot.length l < 256})
+val prepareExtensions: 
+  protocolVersion -> 
+  k:valid_cipher_suites{List.Tot.length k < 256} -> 
+  bool -> 
+  bool -> 
+  list sigHashAlg -> list (x:namedGroup{SEC? x \/ FFDHE? x}) -> 
+  option (TI.cVerifyData * TI.sVerifyData) -> 
+  option CommonDH.keyShare -> 
+  Tot (l:list extension{List.Tot.length l < 256})
 let prepareExtensions pv cs sres sren sigAlgs namedGroups ri ks =
     let res = [] in 
     (* Always send supported extensions. The configuration options will influence how strict the tests will be *)
@@ -474,6 +485,24 @@ let prepareExtensions pv cs sres sren sigAlgs namedGroups ri ks =
     assume (List.Tot.length res < 256);  // JK: Specs in type config in TLSInfo unsufficient
     res
 
+(*
+// TODO the code above is too restrictive, should support further extensions
+// TODO we need an inverse; broken due to extension ordering. Use pure views instead?
+val matchExtensions: list extension{List.Tot.length l < 256} -> Tot ( 
+  protocolVersion *
+  k:valid_cipher_suites{List.Tot.length k < 256} *
+  bool *
+  bool * 
+  list sigHashAlg -> list (x:namedGroup{SEC? x \/ FFDHE? x}) *
+  option (TI.cVerifyData * TI.sVerifyData) *
+  option CommonDH.keyShare )
+let matchExtensions ext = admit()
+
+let prepareExtensions_inverse pv cs sres sren sigAlgs namedGroups ri ks:
+  Lemma(
+    matchExtensions (prepareExtensions pv cs sres sren sigAlgs namedGroups ri ks) =
+    (pv, cs, sres, sren, sigAlgs, namedGroups, ri, ks)) = ()
+*)
 
 (*************************************************
  SI: 
