src/tls/TLSInfo.fst
@@ -290,6 +290,7 @@ type abbrInfo =
      abbr_vd: option (cVerifyData * sVerifyData) }
 
 type resumeInfo (r:role) =
+  //17-04-19  time:lbytes 4  * // initial Nonce.timestamp() for the connection 
   o:option sessionID{r=Server ==> o=None} *
   l:list PSK.psk_identifier {r=Server ==> l = []} // assuming we do the PSK lookups locally
 
